Pushing admits back to smaller lemmas

theories/abs_imp.v
@@ -10,6 +10,7 @@ Section Semantics.
   Context
       (Cs: list CL)
       (Fs: list F)
+      (*name_of should probably be partial to account for non-future ids *)
       (name_of: id -> f)
       (id_of: f -> id)
   .
@@ -28,6 +29,8 @@ Section Semantics.
   | cn_object (C0:C) (a:s) (p:option task) (q: queue)
   | cn_invoc (o0:o) (f0:f) (m0:m) (vs: list t).
 
+  Variant is_fut: cn -> Prop := is_fut_intro: forall f v, is_fut (cn_future f v).
+
   Definition config := (natmap cn).
   Definition add (p:task) (q:queue) := (q ⊎ {[+ p +]}).
   Definition remove (p:task) (q:queue) := (q ∖ {[+ p +]}).
@@ -45,7 +48,17 @@ Section Semantics.
         if String.eqb c name then Some (class name fields methods) else get_class_decl c Cs
     }.
 
-  #[global] Instance elem_of_list_CL: ElemOf C (list CL) := fun c Cs => get_class_decl c Cs <> None.
+  Lemma get_class_decl_some: forall c l C,
+      get_class_decl c l = Some C -> In C l.
+  Proof.
+    induction l; intros; try (now inv H).
+    destruct a.
+    autorewrite with get_class_decl in *.
+    destruct (c =? C5)%string.
+    + inv H.
+      now left.
+    + right; auto.
+  Qed.
 
   Equations bind_params_aux (s0:s) (vs: list t) (params: list (T*x)): s := {
       bind_params_aux s0 [] _ := s0;
@@ -155,243 +168,17 @@ Section Typing.
   Context
       (Cs: list CL)
       (Fs: list F)
+      (*name_of should probably be partial to account for non-future ids *)
       (name_of: id -> f)
       (id_of: f -> id)
       (class_of: o -> C)
   .
 
   Hypothesis (vars_fs_distinct: forall (x_:x) (fn:fc), x_ <> fn).
-
-  Equations typ_es: G -> list e -> list T -> Prop := {
-      typ_es _ [] [] := True ;
-      typ_es Γ (e::es) (T::Ts) := typ_e Γ e T /\ typ_es Γ es Ts ;
-      typ_es _ _ _ := False
-    }.
-
-  Lemma type_preservation_eval: forall Γ,
-      Forall (typ_F Γ) Fs ->
-      forall σ, G_vdash_s Γ σ ->
-           forall e0 e1 T0,
-             typ_e Γ e0 T0 ->
-             eval Fs σ e0 e1 ->
-             typ_e Γ (e_t e1) T0.
-  Proof.
-    intros.
-    destruct H2 as [σ' COMP].
-    pose proof type_preservation vars_fs_distinct  _ _ _ H0 H _ _ _ H1 COMP
-      as (Γ' & SUB & VDASH & TYP).
-    now inv TYP; constructor.
-  Qed.
-
-  Lemma type_preservation_eval_list: forall Γ,
-      Forall (typ_F Γ) Fs ->
-      forall σ, G_vdash_s Γ σ ->
-        forall es vs Ts,
-          typ_es Γ es Ts ->
-          eval_list Fs σ es vs ->
-          typ_es Γ (map e_t vs) Ts.
-  Proof.
-    induction es; intros;
-      destruct vs;
-      destruct Ts;
-      cbn;
-      autorewrite with typ_es eval_list in *;
-      try intuition.
-    eapply type_preservation_eval; eauto.
-  Qed.
-
-  Definition add_G (Γ:G) (Tx:T*x): G := <[Tx.2:=ctxv_T Tx.1]> Γ.
-  Definition extend_G (Γ:G) (l:list (T*x)): G := foldr (flip add_G) Γ l.
-
-  Variant match_method: m -> list T -> T -> CL -> Prop :=
-    match_intro: forall m method Cl,
-        get_method_decl m (get_methods Cl) = Some method ->
-        match_method m (map fst (get_params method)) (get_type method) Cl.
-
-  Variant typ_rhs: G -> rhs -> ctxv -> Prop :=
-    | typ_rhs_e: forall Γ e T,
-        typ_e Γ e T ->
-        typ_rhs Γ (rhs_e e) (ctxv_T T)
-    | typ_rhs_invoc: forall Γ m o es Cl Ts T,
-        typ_es Γ es Ts ->
-        get_class_decl (class_of o) Cs = Some Cl ->
-        match_method m Ts T Cl ->
-        typ_rhs Γ (rhs_invoc o m es) (ctxv_fut T)
-    | typ_rhs_fut: forall Γ f T,
-        Γ !! f = Some (ctxv_fut T) ->
-        typ_rhs Γ (rhs_get f) (ctxv_T T)
-  .
-
-  Inductive stmt_well_typed: G -> stmt -> Prop :=
-  | typ_stmt_seq: forall G s1 s2,
-      stmt_well_typed G s1 ->
-      stmt_well_typed G s2 ->
-      stmt_well_typed G (stmt_seq s1 s2)
-
-  | stmt_well_typed_skip: forall G,
-      stmt_well_typed G stmt_skip
-
-  | stmt_well_typed_asgn: forall G x r T,
-      G !! x = Some T ->
-      typ_rhs G r T ->
-      stmt_well_typed G (stmt_asgn x r)
-
-  | stmt_well_typed_cond: forall G b s1 s2,
-      typ_e G b T_bool ->
-      stmt_well_typed G s1 ->
-      stmt_well_typed G s2 ->
-      stmt_well_typed G (stmt_cond b s1 s2)
-
-  | stmt_well_typed_loop: forall G b s,
-      typ_e G b T_bool ->
-      stmt_well_typed G s ->
-      stmt_well_typed G (stmt_loop b s)
-
-  | stmt_well_typed_return: forall G e T,
-      typ_e G e T ->
-      G !! destiny = Some (ctxv_fut T) ->
-      stmt_well_typed G (stmt_ret e)
-  .
-
-  Variant task_well_typed: G -> option task -> Prop :=
-    | task_wt_idle: forall Γ, task_well_typed Γ None
-    | task_wt: forall Γ stmt l,
-        (* this differs from the paper since we do not treat l as a typed list *)
-        G_vdash_s Γ l ->
-        stmt_well_typed Γ stmt ->
-        task_well_typed Γ (Some (tsk stmt l))
-  .
-
-  Definition queue_well_typed (Γ:G) (q:queue) := forall t, t ∈ q -> task_well_typed Γ (Some t).
-
-  Variant cn_well_typed: G -> cn -> Prop :=
-    | ob_wt: forall Γ c Cl a p q fields,
-        (* The paper also checks fields(Γ(o)), but we would need another case for ctxv *)
-        get_class_decl c Cs = Some Cl ->
-        get_fields Cl = fields ->
-        queue_well_typed (extend_G Γ fields) q ->
-        task_well_typed (extend_G Γ fields) p ->
-        G_vdash_s (extend_G Γ fields) a ->
-        cn_well_typed Γ (cn_object c a p q)
-    | inv_wt: forall Γ o f T Ts m vs Cl,
-        Γ !! f = Some (ctxv_fut T) ->
-        typ_es Γ (map e_t vs) Ts ->
-        get_class_decl (class_of o) Cs = Some Cl ->
-        match_method m Ts T Cl ->
-        cn_well_typed Γ (cn_invoc o f m vs)
-    | fut_wt_none: forall G f T,
-        G !! f = Some (ctxv_fut T) ->
-        cn_well_typed  G (cn_future f None)
-    | fut_wt_some: forall G f t T,
-        G !! f = Some (ctxv_fut T) ->
-        typ_e G (e_t t) T ->
-        cn_well_typed  G (cn_future f (Some t))
-  .
-  Definition config_well_typed (G0:G) (conf: config) :=
-    forall i ob, conf !! i = Some ob -> cn_well_typed G0 ob.
-
-  (** useful tactics and lemmas *)
-
-  Ltac lookup_cases H i j :=
-    is_eq i j; [setoid_rewrite lookup_insert in H; inv H
-               | setoid_rewrite lookup_insert_ne in H; auto].
-
-  Ltac unfold_typing :=
-    repeat (match goal with
-            | H: cn_well_typed _ _ |- _ => inv H
-            | H: task_well_typed _ _ |- _ => inv H
-            | H: stmt_well_typed _ (stmt_seq _ _) |- _ => inv H
-            | H: stmt_well_typed _ (stmt_asgn _ _) |- _ => inv H
-            | H: stmt_well_typed _ (stmt_cond _ _ _) |- _ => inv H
-            | H: stmt_well_typed _ (stmt_loop _ _) |- _ => inv H
-            | H: stmt_well_typed _ (stmt_ret _) |- _ => inv H
-            | H: typ_rhs _ _ _ |- _ => inv H
-            (* | H: match_method _ _ _ _ |- _ => inv H *)
-            end).
-
-  (* should be a theorem, but will require some assumptions on name_of/id_of and typing of futures *)
   Hypothesis id_of_consistent: forall (σ:config) f f' v, σ !! (id_of f) = Some (cn_future f' v) -> f = f'.
-  Variant is_fut: cn -> Prop := is_fut_intro: forall f v, is_fut (cn_future f v).
   Hypothesis id_of_well_typed: forall (σ:config) f c, σ !! (id_of f) = Some c -> is_fut c.
-
-  Lemma fresh_config_wt: forall Γ f σ,
-      fresh f σ -> config_well_typed Γ σ -> f ∉ dom Γ.
-  Proof.
-    unfold fresh, config_well_typed.
-    intros.
-    destruct (σ !! id_of f) eqn:?.
-    - specialize (id_of_well_typed _ _ _ Heqo) as FUT_WT; auto.
-      inv FUT_WT.
-      specialize (H0 _ _ Heqo).
-      specialize (id_of_consistent _ _ _ _ Heqo).
-      intro.
-      eapply H; eauto.
-    - admit.
-      (* this seems problematic *)
-  Admitted.
-
-  Lemma subG_extend: forall Γ l,
-      Forall (fun '(_, x) => x ∉ dom Γ) l ->
-      Γ ⊆ extend_G Γ l.
-  Proof.
-    induction l; intros; auto.
-    destruct a; simpl in *.
-    inv H.
-    eapply subG_add; auto.
-    simpl.
-    now apply not_elem_of_dom.
-  Qed.
-
-  Lemma q_wt_remove: forall  G0 q,
-      queue_well_typed  G0 q ->
-      forall t, queue_well_typed  G0 (remove t q).
-  Proof.
-    intros*.
-    apply H.
-    multiset_solver.
-  Qed.
-
-  Lemma q_wt_add: forall  G0 q,
-      queue_well_typed  G0 q ->
-      forall t,
-        task_well_typed G0 (Some t) ->
-        queue_well_typed  G0 (add t q).
-  Proof.
-    intros*.
-    apply gmultiset_elem_of_disj_union in H1.
-    destruct H1; auto.
-    now apply gmultiset_elem_of_singleton in H1; subst.
-  Qed.
-
-  Lemma G_vdash_union: forall Γ σ σ',
-      G_vdash_s Γ σ ->
-      (* somewhat surprisingly we do not need σ' because map_union prefers the left*)
-      (* G_vdash_s Γ σ' -> *)
-      G_vdash_s Γ (union σ σ').
-  Proof.
-    intros*.
-    apply H in H0.
-    destruct H0 as (?t & LU & TYP).
-    exists t.
-    split; simp; auto.
-  Qed.
-
-  (* this is a problem: well-typing of tasks is not closed under extensions *)
-  Fact subG_task_wt : exists Γ1 Γ2 t,
-      Γ1 ⊆ Γ2 /\ task_well_typed  Γ1 t /\ ~ task_well_typed  Γ2 t.
-  Proof.
-    exists ∅, (<["x":=ctxv_T T_bool]> ∅), (Some (tsk stmt_skip (<["x":=t_int Z0]> ∅))).
-    splits.
-    - now apply insert_subseteq.
-    - econstructor.
-      + intros*.
-        inv H.
-      + constructor.
-    - inv 1.
-      pose proof H3 "x" (ctxv_T T_bool) as (?t' & ? & ?); auto.
-      simpl in H0.
-      inv H0.
-  Qed.
+  Hypothesis id_of_name_of: forall i, id_of (name_of i) = i.
+  Hypothesis name_of_id_of: forall f, name_of (id_of f) = f.
 
   (* this substitution and subsequent well-typing is not currently used *)
   (* I thought I might use it, and then didn't, but may be useful later? *)
@@ -437,6 +224,325 @@ Section Typing.
     inv H; constructor.
   Qed.
 
+  Equations typ_es: G -> list e -> list T -> Prop := {
+      typ_es _ [] [] := True ;
+      typ_es Γ (e::es) (T::Ts) := typ_e Γ e T /\ typ_es Γ es Ts ;
+      typ_es _ _ _ := False
+    }.
+
+  Lemma typ_term_invariant: forall Γ v T,
+      typ_e Γ (e_t v) T ->
+      forall Γ',
+        typ_e Γ' (e_t v) T.
+  Proof.
+    intros.
+    inv H; constructor.
+  Qed.
+
+  Lemma typ_term_list_invariant: forall Γ vs Ts,
+      typ_es Γ (map e_t vs) Ts ->
+      forall Γ',
+        typ_es Γ' (map e_t vs) Ts.
+    Proof.
+      induction vs; destruct Ts; intros; auto.
+      simpl in *.
+      autorewrite with typ_es in *.
+      destruct H.
+      split; auto.
+      eapply typ_term_invariant; eauto.
+    Qed.
+
+  Lemma type_preservation_eval: forall Γ,
+      Forall (typ_F Γ) Fs ->
+      forall σ, G_vdash_s Γ σ ->
+           forall e0 e1 T0,
+             typ_e Γ e0 T0 ->
+             eval Fs σ e0 e1 ->
+             typ_e Γ (e_t e1) T0.
+  Proof.
+    intros.
+    destruct H2 as [σ' COMP].
+    pose proof type_preservation vars_fs_distinct  _ _ _ H0 H _ _ _ H1 COMP
+      as (Γ' & SUB & VDASH & TYP).
+    now inv TYP; constructor.
+  Qed.
+
+  Lemma type_preservation_eval_list: forall Γ,
+      Forall (typ_F Γ) Fs ->
+      forall σ, G_vdash_s Γ σ ->
+        forall es vs Ts,
+          typ_es Γ es Ts ->
+          eval_list Fs σ es vs ->
+          typ_es Γ (map e_t vs) Ts.
+  Proof.
+    induction es; intros;
+      destruct vs;
+      destruct Ts;
+      cbn;
+      autorewrite with typ_es eval_list in *;
+      try intuition.
+    eapply type_preservation_eval; eauto.
+  Qed.
+
+  Definition add_G (Γ:G) (Tx:T*x): G := <[Tx.2:=ctxv_T Tx.1]> Γ.
+  Definition extend_G (Γ:G) (l:list (T*x)): G := foldr (flip add_G) Γ l.
+
+  Lemma extend_subG: forall Γ1 Γ2 l,
+      Γ1 ⊆ Γ2 -> extend_G Γ1 l ⊆ extend_G Γ2 l.
+  Proof.
+    induction l; intros; auto.
+    destruct a; simpl.
+    apply insert_mono.
+    now apply IHl.
+  Qed.
+
+  Lemma subG_extend: forall Γ l,
+      Forall (fun '(_, x) => x ∉ dom Γ) l ->
+      Γ ⊆ extend_G Γ l.
+  Proof.
+    induction l; intros; auto.
+    destruct a; simpl in *.
+    inv H.
+    eapply subG_add; auto.
+    simpl.
+    now apply not_elem_of_dom.
+  Qed.
+
+  Lemma addG_subG: forall Γ1 Γ2 Tx,
+      add_G Γ1 Tx ⊆ Γ2 ->
+      Tx.2 ∉ dom Γ1 ->
+      Γ1 ⊆ Γ2.
+  Proof.
+    unfold add_G.
+    intros.
+    epose proof map_subseteq_spec _ _ as (? & _).
+    pose proof H as H'.
+    eapply H1 with (i:=Tx.2) in H; last eapply lookup_insert.
+    eapply subG_add_2 in H; eauto.
+    transitivity (<[Tx.2:=ctxv_T Tx.1]> Γ1); auto.
+    apply subG_add; auto.
+    now apply not_elem_of_dom.
+  Qed.
+
+  Lemma extend_domain: forall Γ x l,
+      x ∉ dom Γ ->
+      Forall (λ '(_, x0), x0 <> x) l ->
+      x ∉ dom (extend_G Γ l).
+  Proof.
+    induction l; intros; auto.
+    destruct a; simpl in *.
+    inv H0.
+    pose proof IHl H H4.
+    apply not_elem_of_dom.
+    setoid_rewrite lookup_insert_ne; auto.
+    now apply not_elem_of_dom.
+  Qed.
+
+  Lemma extend_subG_2: forall Γ1 Γ2 l,
+      extend_G Γ1 l ⊆ Γ2 ->
+      Forall (λ '(_, x), x ∉ dom Γ2) l ->
+      Γ1 ⊆ Γ2.
+  Proof.
+    induction l; intros; auto.
+    destruct a; simpl in *.
+    inv H0.
+    apply addG_subG in H; auto.
+    apply extend_domain; auto.
+    - eapply lookup_weaken with (i:=x) in H; last apply lookup_insert.
+      apply not_elem_of_dom in H3.
+      setoid_rewrite H3 in H.
+      inv H.
+    - apply Forall_forall.
+      intros (?&?) ? ?.
+      eapply Forall_forall in H4; eauto.
+      simpl in *; subst.
+      eapply lookup_weaken with (i:=x) in H; last apply lookup_insert.
+      apply not_elem_of_dom in H3.
+      setoid_rewrite H3 in H.
+      inv H.
+   Qed.
+
+  Variant match_method: m -> list T -> T -> CL -> Prop :=
+    match_intro: forall m method Cl,
+        get_method_decl m (get_methods Cl) = Some method ->
+        match_method m (map fst (get_params method)) (get_type method) Cl.
+
+  Variant typ_rhs: G -> rhs -> ctxv -> Prop :=
+    | typ_rhs_e: forall Γ e T,
+        typ_e Γ e T ->
+        typ_rhs Γ (rhs_e e) (ctxv_T T)
+    | typ_rhs_invoc: forall Γ m o es Cl Ts T,
+        typ_es Γ es Ts ->
+        get_class_decl (class_of o) Cs = Some Cl ->
+        match_method m Ts T Cl ->
+        typ_rhs Γ (rhs_invoc o m es) (ctxv_T T)
+    | typ_rhs_get: forall Γ f T,
+        Γ !! f = Some (ctxv_fut T) ->
+        typ_rhs Γ (rhs_get f) (ctxv_T T)
+  .
+
+  Inductive stmt_well_typed: G -> stmt -> Prop :=
+  | typ_stmt_seq: forall G s1 s2,
+      stmt_well_typed G s1 ->
+      stmt_well_typed G s2 ->
+      stmt_well_typed G (stmt_seq s1 s2)
+
+  | stmt_well_typed_skip: forall G,
+      stmt_well_typed G stmt_skip
+
+  | stmt_well_typed_asgn: forall G x r T,
+      G !! x = Some T ->
+      typ_rhs G r T ->
+      stmt_well_typed G (stmt_asgn x r)
+
+  | stmt_well_typed_cond: forall G b s1 s2,
+      typ_e G b T_bool ->
+      stmt_well_typed G s1 ->
+      stmt_well_typed G s2 ->
+      stmt_well_typed G (stmt_cond b s1 s2)
+
+  | stmt_well_typed_loop: forall G b s,
+      typ_e G b T_bool ->
+      stmt_well_typed G s ->
+      stmt_well_typed G (stmt_loop b s)
+
+  | stmt_well_typed_return: forall G e T,
+      typ_e G e T ->
+      G !! destiny = Some (ctxv_fut T) ->
+      stmt_well_typed G (stmt_ret e)
+  .
+
+  Variant task_well_typed: G -> option task -> Prop :=
+    | task_wt_idle: forall Γ, task_well_typed Γ None
+    | task_wt: forall Γ stmt l,
+        (* this differs from the paper since we do not treat l as a typed list *)
+        (* G_vdash_s Γ l -> *)
+        stmt_well_typed Γ stmt ->
+        task_well_typed Γ (Some (tsk stmt l))
+  .
+
+  Definition queue_well_typed (Γ:G) (q:queue) := forall t, t ∈ q -> task_well_typed Γ (Some t).
+
+  Variant cn_well_typed: G -> cn -> Prop :=
+    | ob_wt: forall Γ c Cl a p q fields,
+        (* The paper also checks fields(Γ(o)), but we would need another case for ctxv *)
+        get_class_decl c Cs = Some Cl ->
+        get_fields Cl = fields ->
+        queue_well_typed (extend_G Γ fields) q ->
+        task_well_typed (extend_G Γ fields) p ->
+        G_vdash_s (extend_G Γ fields) a ->
+        cn_well_typed Γ (cn_object c a p q)
+    | inv_wt: forall Γ o f T Ts m vs Cl,
+        Γ !! f = Some (ctxv_fut T) ->
+        typ_es Γ (map e_t vs) Ts ->
+        get_class_decl (class_of o) Cs = Some Cl ->
+        match_method m Ts T Cl ->
+        cn_well_typed Γ (cn_invoc o f m vs)
+    | fut_wt_none: forall G f T,
+        G !! f = Some (ctxv_fut T) ->
+        cn_well_typed  G (cn_future f None)
+    | fut_wt_some: forall G f t T,
+        G !! f = Some (ctxv_fut T) ->
+        typ_e G (e_t t) T ->
+        cn_well_typed  G (cn_future f (Some t))
+  .
+  Definition config_well_typed (G0:G) (conf: config) :=
+    forall i ob, conf !! i = Some ob -> cn_well_typed G0 ob.
+
+  Example typing_get: let Γ := (<["x":=ctxv_T T_int]> (<["f":=ctxv_fut T_int]> ∅)) in
+                      stmt_well_typed Γ (stmt_asgn "x" (rhs_get "f")).
+  Proof.
+    apply stmt_well_typed_asgn with (ctxv_T T_int); auto.
+    apply typ_rhs_get; auto.
+  Qed.
+
+  (** useful tactics and lemmas *)
+
+  Ltac lookup_cases H i j :=
+    is_eq i j; [setoid_rewrite lookup_insert in H; inv H
+               | setoid_rewrite lookup_insert_ne in H; auto].
+
+  Ltac unfold_typing :=
+    repeat (match goal with
+            | H: cn_well_typed _ _ |- _ => inv H
+            | H: task_well_typed _ _ |- _ => inv H
+            | H: stmt_well_typed _ (stmt_seq _ _) |- _ => inv H
+            | H: stmt_well_typed _ (stmt_asgn _ _) |- _ => inv H
+            | H: stmt_well_typed _ (stmt_cond _ _ _) |- _ => inv H
+            | H: stmt_well_typed _ (stmt_loop _ _) |- _ => inv H
+            | H: stmt_well_typed _ (stmt_ret _) |- _ => inv H
+            | H: typ_rhs _ _ _ |- _ => inv H
+            (* | H: match_method _ _ _ _ |- _ => inv H *)
+            end).
+
+  (* should be a theorem, but will require some assumptions on name_of/id_of and typing of futures *)
+  Lemma fresh_config_wt: forall Γ f σ,
+      fresh f σ -> config_well_typed Γ σ -> f ∉ dom Γ.
+  Proof.
+    unfold fresh, config_well_typed.
+    intros.
+    destruct (σ !! id_of f) eqn:?.
+    - specialize (id_of_well_typed _ _ _ Heqo) as FUT_WT; auto.
+      inv FUT_WT.
+      specialize (H0 _ _ Heqo).
+      specialize (id_of_consistent _ _ _ _ Heqo).
+      intro.
+      eapply H; eauto.
+    - admit.
+      (* this seems problematic *)
+  Admitted.
+
+  Lemma q_wt_remove: forall  G0 q,
+      queue_well_typed  G0 q ->
+      forall t, queue_well_typed  G0 (remove t q).
+  Proof.
+    intros*.
+    apply H.
+    multiset_solver.
+  Qed.
+
+  Lemma q_wt_add: forall  G0 q,
+      queue_well_typed  G0 q ->
+      forall t,
+        task_well_typed G0 (Some t) ->
+        queue_well_typed  G0 (add t q).
+  Proof.
+    intros*.
+    apply gmultiset_elem_of_disj_union in H1.
+    destruct H1; auto.
+    now apply gmultiset_elem_of_singleton in H1; subst.
+  Qed.
+
+  Lemma G_vdash_union: forall Γ σ σ',
+      G_vdash_s Γ σ ->
+      (* somewhat surprisingly we do not need σ' because map_union prefers the left*)
+      (* G_vdash_s Γ σ' -> *)
+      G_vdash_s Γ (union σ σ').
+  Proof.
+    intros*.
+    apply H in H0.
+    destruct H0 as (?t & LU & TYP).
+    exists t.
+    split; simp; auto.
+  Qed.
+
+  (* this is a problem: well-typing of tasks is not closed under extensions *)
+  (* Fact subG_task_wt : exists Γ1 Γ2 t, *)
+  (*     Γ1 ⊆ Γ2 /\ task_well_typed  Γ1 t /\ ~ task_well_typed  Γ2 t. *)
+  (* Proof. *)
+  (*   exists ∅, (<["x":=ctxv_T T_bool]> ∅), (Some (tsk stmt_skip (<["x":=t_int Z0]> ∅))). *)
+  (*   splits. *)
+  (*   - now apply insert_subseteq. *)
+  (*   - econstructor. *)
+  (*     + intros*. *)
+  (*       inv H. *)
+  (*     + constructor. *)
+  (*   - inv 1. *)
+  (*     pose proof H3 "x" (ctxv_T T_bool) as (?t' & ? & ?); auto. *)
+  (*     simpl in H0. *)
+  (*     inv H0. *)
+  (* Qed. *)
+
   Lemma subG_typ_es: forall G1 G2 es Ts,
       subseteq G1 G2 -> typ_es G1 es Ts -> typ_es G2 es Ts.
   Proof.
@@ -478,60 +584,193 @@ Section Typing.
       + eapply lookup_weaken; eauto.
   Qed.
 
+  Lemma subG_task_wt : forall Γ1 Γ2 t,
+      Γ1 ⊆ Γ2 -> task_well_typed  Γ1 t -> task_well_typed  Γ2 t.
+  Proof.
+    intros.
+    destruct t.
+    - destruct t.
+      constructor.
+      inv H0.
+      eapply subG_stmt_wt; eauto.
+    - constructor.
+  Qed.
+
+  Lemma subG_queue_wt : forall Γ1 Γ2 q,
+      Γ1 ⊆ Γ2 -> queue_well_typed  Γ1 q -> queue_well_typed  Γ2 q.
+  Proof.
+    intros*.
+    eapply subG_task_wt; eauto.
+  Qed.
+
   Lemma fresh_extend_wt: forall Γ σ f,
       config_well_typed Γ σ ->
       fresh f σ ->
       forall T_,
         config_well_typed (<[f:=T_]> Γ) σ.
   Proof.
+    intros.
+    intros i ob LUi.
+    remember (id_of f) as fi.
+    is_eq i fi; subst.
+    - pose proof id_of_well_typed _ _ _ LUi as FUT.
+      inv FUT.
+      pose proof H0 _ _ _ LUi.
+      pose proof id_of_consistent _ _ _ _ LUi as <- .
+      contradiction.
+    - epose proof H i ob LUi.
+      destruct ob.
+      + enough (diff : f <> f0).
+        {
+        destruct v.
+        - inv H1.
+          econstructor; auto.
+          + setoid_rewrite lookup_insert_ne; eauto.
+          + inv H6; constructor.
+        - inv H1.
+          econstructor.
+          setoid_rewrite lookup_insert_ne; eauto.
+        }
+        intro.
+        replace i with (id_of (name_of i)) in *
+            by apply id_of_name_of.
+        pose proof id_of_consistent _ _ _ _ LUi.
+        subst.
+        contradiction.
+      + admit.
+      (* adding a future to the context does not impact typing of an object *)
+      + admit.
+        (* for invocations it is less obvious *)
+  Admitted.
+
+  Lemma bind_wt: forall m Ts T CL vs f tsk,
+      match_method m Ts T CL ->
+      bind m vs f CL = tsk ->
+      forall Γ,
+        Γ !! f = Some (ctxv_fut T) ->
+        typ_es Γ (map e_t vs) Ts ->
+        task_well_typed Γ tsk.
+  Proof.
+  Admitted.
+
+  Lemma insert_lookup_ne_extend: forall Γ i j T_ l,
+      i <> j ->
+      extend_G (<[j:=T_]> Γ) l !! i = extend_G Γ l !! i.
+  Proof.
+    induction l; intros; simpl.
+    - now apply lookup_insert_ne.
+    - unfold add_G; destruct a; simpl.
+      is_eq i x.
+      + now setoid_rewrite lookup_insert.
+      + setoid_rewrite lookup_insert_ne; eauto.
+  Qed.
+
+  Definition CL_well_typed: G -> CL -> Prop := fun _ _ => True. (*TODO: implement*)
+
+  Lemma CL_wt_fields_fresh: forall Γ C,
+      CL_well_typed Γ C ->
+      Forall (λ '(_, x), x ∉ dom Γ) (get_fields C).
+  Admitted.
+  (* arguably too strong, we only really need them to agree *)
+  (* replace subG_extend with a weaker version *)
+
+  Lemma CL_wt_add_f: forall Γ C (f:f) T,
+      CL_well_typed Γ C ->
+      CL_well_typed (<[f:=T]> Γ) C.
+  Admitted.
+
+  Lemma Forall_typ_F_extension: forall Γ Fs Cl,
+      Forall (typ_F Γ) Fs ->
+      Forall (CL_well_typed Γ) Cs ->
+      In Cl Cs ->
+      Forall (typ_F (extend_G Γ (get_fields Cl))) Fs.
   Admitted.
 
   Theorem type_preservation : forall (Γ: G),
       Forall (typ_F Γ) Fs ->
+      Forall (CL_well_typed Γ) Cs ->
       forall σ σ',
         config_well_typed Γ σ ->
         stmt_step Cs Fs id_of σ σ' ->
         exists Γ', Γ ⊆ Γ' /\ config_well_typed Γ' σ'.
   Proof.
-    intros.
-    inv H1.
+    intros Γ TYP_Fs TYP_Cs σ σ' WT STEP.
+    inv STEP.
     - exists Γ; split; auto.
       intros*.
       lookup_cases H1 i i0.
-      + specialize (H0 _ _ H3).
+      + specialize (WT _ _ H0).
         unfold_typing.
         destruct p.
         econstructor; eauto.
         now apply q_wt_remove.
-      + eapply H0;eauto.
+      + eapply WT;eauto.
 
-    - destruct H3 as [sf ?].
-      pose proof H1 as Conf_wt.
-      specialize (H0 _ _ H4).
+    - destruct H0 as [sf ?].
+      pose proof WT as Conf_wt.
+      specialize (WT _ _ H1).
       unfold_typing.
-      epose proof type_preservation _ _ _ _ _ _ _ _ _ H5 H1
+      epose proof type_preservation _ _ _ _ _ _ _ _ _ H4 H0
         as (?Γ & ?SUB & ? & ?TYP_E).
       (* are tasks actually well-typed under this extension? *)
-      admit.
-      Unshelve.
-      + apply vars_fs_distinct.
-      + now apply G_vdash_union.
-      + apply subG_typ_F_forall with Γ; auto.
-        apply subG_extend.
-        admit. (* can we guarantee that the fields are not already in the context? *)
+      eexists.
+      split; eauto.
+      intros*.
+      lookup_cases H3 i i0.
+      + econstructor; eauto.
+        econstructor; eauto.
+      + eapply Conf_wt; eauto.
 
-    - destruct H3 as [sf ?].
-      pose proof H1 as Conf_wt.
-      specialize (H0 _ _ H4).
+    - destruct H0 as [sf ?].
+      pose proof WT as Conf_wt.
+      specialize (WT _ _ H1).
       unfold_typing.
-      epose proof type_preservation _ _ _ _ _ _ _ _ _ H5 H1
+      epose proof type_preservation _ _ _ _ _ _ _ _ _ H4 H0
         as (?Γ & ?SUB & ? & ?TYP_E).
-      admit.
+      exists Γ0.
+      split.
+      + eapply extend_subG_2; eauto.
+        apply CL_wt_fields_fresh.
+        eapply Forall_forall; eauto.
+        eapply get_class_decl_some; eauto.
+      + intros*.
+        lookup_cases H3 o i.
+        * assert (extend_G Γ (get_fields Cl) ⊆ extend_G Γ0 (get_fields Cl)). {
+             eapply extend_subG.
+             eapply extend_subG_2; eauto.
+             apply CL_wt_fields_fresh.
+             eapply Forall_forall; eauto.
+             eapply get_class_decl_some; eauto.
+            }
+          econstructor; eauto.
+          -- eapply subG_queue_wt; eauto.
+          -- constructor.
+             eapply subG_stmt_wt; eauto.
+          -- admit. (* here we are lost without consistency of a *)
+        * admit. (* we need cn_well_typed closed under extensions *)
 
     (* the trivial cases (ifs, skips, loops) are very similar*)
     (* TODO: automate *)
-    - pose proof H0 as Conf_wt.
-      specialize (H0 _ _ H3).
+    - pose proof WT as Conf_wt.
+      specialize (WT _ _ H0).
+      unfold_typing.
+      exists Γ; split; auto.
+      intros*.
+      lookup_cases H1 o i.
+      + repeat (econstructor; eauto).
+      + eapply Conf_wt; eauto.
+
+    - pose proof WT as Conf_wt.
+      specialize (WT _ _ H0).
+      unfold_typing.
+      exists Γ; split; auto.
+      intros*.
+      lookup_cases H1 o i.
+      + repeat (econstructor; eauto).
+      + eapply Conf_wt; eauto.
+
+    - pose proof WT as Conf_wt.
+      specialize (WT _ _ H).
       unfold_typing.
       exists Γ; split; auto.
       intros*.
@@ -539,8 +778,8 @@ Section Typing.
       + repeat (econstructor; eauto).
       + eapply Conf_wt; eauto.
 
-    - pose proof H0 as Conf_wt.
-      specialize (H0 _ _ H3).
+    - pose proof WT as Conf_wt.
+      specialize (WT _ _ H).
       unfold_typing.
       exists Γ; split; auto.
       intros*.
@@ -548,8 +787,8 @@ Section Typing.
       + repeat (econstructor; eauto).
       + eapply Conf_wt; eauto.
 
-    - pose proof H0 as Conf_wt.
-      specialize (H0 _ _ H2).
+    - pose proof WT as Conf_wt.
+      specialize (WT _ _ H).
       unfold_typing.
       exists Γ; split; auto.
       intros*.
@@ -557,127 +796,147 @@ Section Typing.
       + repeat (econstructor; eauto).
       + eapply Conf_wt; eauto.
 
-    - pose proof H0 as Conf_wt.
-      specialize (H0 _ _ H2).
+    - pose proof WT as Conf_wt.
+      specialize (WT _ _ H2).
       unfold_typing.
-      exists Γ; split; auto.
-      intros*.
-      lookup_cases H0 o i.
-      + repeat (econstructor; eauto).
-      + eapply Conf_wt; eauto.
-
-    - pose proof H0 as Conf_wt.
-      specialize (H0 _ _ H2).
-      unfold_typing.
-      exists Γ; split; auto.
-      intros*.
-      lookup_cases H0 o i.
-      + repeat (econstructor; eauto).
-      + eapply Conf_wt; eauto.
-
-    - pose proof H0 as Conf_wt.
-      specialize (H0 _ _ H5).
-      unfold_typing.
-      pose proof H18 as Method_wt.
-      inv H18.
+      pose proof H16 as Method_wt.
+      inv H16.
       destruct method.
       autorewrite with get_type get_params in *.
-      epose proof type_preservation_eval_list _ _ _ _ _ _ _ H15 H4 as TYP_ARGS.
+      epose proof type_preservation_eval_list _ _ _ _ _ _ _ H13 H1 as TYP_ARGS.
       exists (<[f:=ctxv_fut T_5]> Γ).
       split.
       + apply subG_add; auto.
         apply not_elem_of_dom.
         eapply fresh_config_wt; eauto.
       + intros*.
-        lookup_cases H1 oi i0.
+        lookup_cases H4 oi i0.
         * econstructor; eauto.
-          -- admit.
-          -- constructor; auto.
-             ++ admit.
-             ++ econstructor.
-                ** econstructor; eauto.
-                   --- admit.
-                   --- econstructor.
-                       eapply lookup_weaken with (<[f:=ctxv_fut T_5]> Γ).
-                       +++ apply lookup_insert.
-                       +++ apply subG_extend.
-                           admit.
-                ** eapply subG_stmt_wt.
-                   --- admit.
-                   --- eauto.
+          -- eapply subG_queue_wt; last apply H10.
+             eapply extend_subG.
+             apply subG_add; auto.
+             apply not_elem_of_dom_1.
+             eapply fresh_config_wt; eauto.
+          -- constructor.
+             econstructor.
+             ++ econstructor; eauto.
+                ** rewrite insert_lookup_ne_extend; eauto.
+                ** econstructor.
+                   eapply lookup_weaken with (<[f:=ctxv_fut T_5]> Γ).
+                   --- now setoid_rewrite lookup_insert.
+                   --- apply subG_extend.
+                       apply CL_wt_fields_fresh.
+                       apply CL_wt_add_f.
+                       eapply Forall_forall; eauto.
+                       eapply get_class_decl_some; eauto.
+             ++ eapply subG_stmt_wt; last apply H9.
+                eapply extend_subG.
+                apply subG_add; auto.
+                apply not_elem_of_dom_1.
+                eapply fresh_config_wt; eauto.
           -- admit. (* should follow from freshness *)
-        * lookup_cases H1 i i0.
+
+        * lookup_cases H4 i i0.
           -- econstructor; eauto.
              ++ apply lookup_insert.
-             ++ admit. (* I would like to use TYP_ARGS, but that includes the fields from the object *)
+             ++ eapply typ_term_list_invariant; eauto.
           -- set (fi:=id_of f).
              is_eq fi i0; subst fi.
-             ++ setoid_rewrite lookup_insert in H1.
-                inv H1.
+             ++ setoid_rewrite lookup_insert in H4.
+                inv H4.
                 econstructor.
                 apply lookup_insert.
-             ++ setoid_rewrite lookup_insert_ne in H1; auto.
+             ++ setoid_rewrite lookup_insert_ne in H4; auto.
                 eapply fresh_extend_wt; eauto.
 
-    - pose proof H0 _ _ H3 as fut_well_typed.
-      pose proof H0 _ _ H4 as ob_well_typed.
+    - pose proof WT _ _ H0 as fut_well_typed.
+      pose proof WT _ _ H1 as ob_well_typed.
       exists Γ; split; auto.
       intros*.
       unfold_typing.
-      lookup_cases H1 o i.
+      lookup_cases H3 o i.
       + econstructor; eauto.
         econstructor.
-      + lookup_cases H1 fi i.
+      + lookup_cases H3 fi i.
         * econstructor; eauto.
-          epose proof type_preservation_eval _ _ _ _ _ _ _ H7 H2.
-          enough (T0 = T) by (subst; inv H1; constructor).
-          pose proof (H11 _ _ H14) as (?t & ? & ?); simp.
-          inv H1; inv H9.
-        * eapply H0; eauto.
+          epose proof type_preservation_eval _ _ _ _ _ _ _ H5 H.
+          enough (T0 = T) by (subst; inv H3; constructor).
+          (* now we have a problem since the local state is not required to be consistent *)
+          (* pose proof (H15 _ _ H5) as (?t & ? & ?); simp. *)
+          (* inv H1; inv H9. *)
+          admit.
+        * eapply WT; eauto.
 
-    - pose proof H0 _ _ H2 as fut_well_typed.
-      pose proof H0 _ _ H3 as ob_well_typed.
+    - pose proof WT _ _ H as fut_well_typed.
+      pose proof WT _ _ H0 as ob_well_typed.
       exists Γ; split; auto.
       intros*.
       unfold_typing.
       lookup_cases H1 o i.
       + repeat (econstructor; eauto).
-        replace T1 with T by admit. (* follows from f ∉ fields(Cl) *)
-        eapply subG_type with Γ; auto.
+        enough (T1 = T) by (subst; eapply typ_term_invariant; eauto).
+        eapply lookup_weaken with (m2:=extend_G Γ (get_fields Cl)) in H5.
+        now simp.
         apply subG_extend.
-        admit.
-      + eapply H0; eauto.
+        apply CL_wt_fields_fresh.
+        eapply Forall_forall; eauto.
+        eapply get_class_decl_some; eauto.
+      + eapply WT; eauto.
 
-    - pose proof H0 _ _ H2 as ob_well_typed.
-      pose proof H0 _ _ H3 as inv_well_typed.
+    - pose proof WT _ _ H as ob_well_typed.
+      pose proof WT _ _ H0 as inv_well_typed.
       exists Γ; split; auto.
       intros*.
       unfold_typing.
-      + lookup_cases H1 oi i0.
+      + lookup_cases H2 oi i0.
         * repeat (econstructor; eauto).
           apply q_wt_add; auto.
-          admit. (* here we need Γ ⊢ Cl -> Γ ⊢ bind m vs f*)
+          replace CL with Cl in * by admit. (* by welformedness of class_of, probably *)
+          eapply bind_wt; eauto.
+          -- apply lookup_weaken with Γ; auto.
+             apply subG_extend.
+             apply CL_wt_fields_fresh.
+             eapply Forall_forall; eauto.
+             eapply get_class_decl_some; eauto.
+          -- eapply subG_typ_es; last apply H10.
+             apply subG_extend.
+             apply CL_wt_fields_fresh.
+             eapply Forall_forall; eauto.
+             eapply get_class_decl_some; eauto.
         * is_eq i i0.
           -- exfalso.
-             setoid_rewrite (lookup_delete σ i) in H1.
-             inv H1.
-          -- setoid_rewrite lookup_delete_ne in H1; auto.
-             eapply H0; eauto.
-      + lookup_cases H1 oi i0.
+             setoid_rewrite (lookup_delete σ i) in H2.
+             inv H2.
+          -- setoid_rewrite lookup_delete_ne in H2; auto.
+             eapply WT; eauto.
+      + lookup_cases H2 oi i0.
         * repeat (econstructor; eauto).
           apply q_wt_add; auto.
-          admit. (* here we need Γ ⊢ Cl -> Γ ⊢ bind m vs f*)
+          replace CL with Cl in * by admit. (* by welformedness of class_of, probably *)
+          eapply bind_wt; eauto.
+          -- apply lookup_weaken with Γ; auto.
+             apply subG_extend.
+             apply CL_wt_fields_fresh.
+             eapply Forall_forall; eauto.
+             eapply get_class_decl_some; eauto.
+          -- eapply subG_typ_es; last apply H10.
+             apply subG_extend.
+             apply CL_wt_fields_fresh.
+             eapply Forall_forall; eauto.
+             eapply get_class_decl_some; eauto.
+
         * is_eq i i0.
           -- exfalso.
-             setoid_rewrite (lookup_delete σ i) in H1.
-             inv H1.
-          -- setoid_rewrite lookup_delete_ne in H1; auto.
-             eapply H0; eauto.
+             setoid_rewrite (lookup_delete σ i) in H2.
+             inv H2.
+          -- setoid_rewrite lookup_delete_ne in H2; auto.
+             eapply WT; eauto.
 
              Unshelve.
              all: try eauto.
              all: try (now apply G_vdash_union).
-             (*remaining: typ_F closed under (well-typed?) extensions *)
+             all: apply Forall_typ_F_extension; auto;
+               eapply get_class_decl_some; eauto.
   Admitted.
 End Typing.
 (*TODO: labels + traces? *)
